Add get_mode in top-level interface for Barry

src/tls/Handshake.fst
@@ -96,6 +96,7 @@ let random_of (s:hs) = nonce s
 let config_of (s:hs) = Nego.local_config s.nego
 let version_of (s:hs) = Nego.version s.nego
 let resumeInfo_of (s:hs) = Nego.resume s.nego
+let get_mode (s:hs) = Nego.getMode s.nego
 let epochs_of (s:hs) = s.epochs
 
 (* WIP on the handshake invariant
